Kami/Ex/FifoCorrect.v
@@ -7,6 +7,8 @@ Require Import Ex.Fifo Ex.NativeFifo Lia.
 
 Import ListNotations.
 
+#[local] Arguments Stdlib.ZArith.BinInt.Z.pow : simpl never.
+#[local] Arguments Stdlib.ZArith.BinInt.Z.of_nat : simpl never.
 Set Implicit Arguments.
 Set Asymmetric Patterns.
 #[warning="-unknown-option"] Set Asymmetric Patterns No Implicits.
